theories/asm.v
@@ -49,7 +49,7 @@ Add Printing Constructor asm_state.
 Definition initial_asm_state (instrs : gmap Z asm_instr) := AsmState AWaiting ∅ ∅ instrs.
 
 Inductive asm_ev :=
-| EAJump (pc : Z) (regs : gmap string Z) (mem : gmap Z (option Z))
+| EAJump (regs : gmap string Z) (mem : gmap Z (option Z))
 | EASyscallCall (args : list Z)
 | EASyscallRet (ret : Z)
 | EAPagefault (a : Z)
@@ -95,13 +95,13 @@ Inductive asm_step : asm_state → option asm_event → (asm_state → Prop) →
 | SJumpExternal regs instrs pc mem:
   regs !!! "PC" = pc →
   instrs !! pc = None →
-  asm_step (AsmState (ARunning []) regs mem instrs) (Some (Outgoing, EAJump pc regs mem))
+  asm_step (AsmState (ARunning []) regs mem instrs) (Some (Outgoing, EAJump regs mem))
            (λ σ', σ' = AsmState AWaiting regs mem instrs)
 | SRecvJump regs regs' instrs pc es mem mem':
   regs' !!! "PC" = pc →
   instrs !! pc = Some es →
   asm_step (AsmState AWaiting regs mem instrs)
-           (Some (Incoming, EAJump pc regs' mem'))
+           (Some (Incoming, EAJump regs' mem'))
            (* We use [] here such that each instruction starts from [] *)
            (λ σ', σ' = AsmState (ARunning []) regs' mem' instrs)
 | SPagefaulting regs instrs a mem:
@@ -128,7 +128,7 @@ Global Hint Resolve asm_step_WriteReg_i : tstep.
 
 Lemma asm_step_WriteReg_s r f es rs ins mem:
   TStepS asm_module (AsmState (ARunning (WriteReg r f::es)) rs mem ins)
-            (λ G, G None (λ G', G' (AsmState (ARunning (es)) (<[r:=f rs]>rs) mem ins))).
+            (λ G, G None (λ G', G' (AsmState (ARunning es) (<[r:=f rs]>rs) mem ins))).
 Proof.
   constructor => ??. eexists _, _. split; [done|] => ? /= ?.
   apply: steps_spec_step_end. { econs. }
@@ -243,7 +243,7 @@ Lemma asm_step_Jump_i rs ins mem:
           if ins !! pc is Some i then
             G true None (λ G', G' (AsmState (ARunning i) rs mem ins))
           else
-            G true (Some (Outgoing, EAJump pc rs mem)) (λ G', G' (AsmState AWaiting rs mem ins))
+            G true (Some (Outgoing, EAJump rs mem)) (λ G', G' (AsmState AWaiting rs mem ins))
    ).
 Proof.
   constructor => ? HG. apply steps_impl_step_end => ???.
@@ -258,7 +258,7 @@ Lemma asm_step_Jump_s rs ins mem:
       if ins !! pc is Some i then
         G None (λ G', G' (AsmState (ARunning i) rs mem ins))
       else
-        G (Some (Outgoing, EAJump pc rs mem)) (λ G', G' (AsmState AWaiting rs mem ins))).
+        G (Some (Outgoing, EAJump rs mem)) (λ G', G' (AsmState AWaiting rs mem ins))).
 Proof.
   constructor => ?[?[??]]. case_match.
   all: eexists _, _; split; [done|] => ? /= ?.
@@ -271,7 +271,7 @@ Lemma asm_step_AWaiting_i rs ins mem:
     ∀ pc i rs' mem',
       rs' !!! "PC" = pc →
       ins !! pc = Some i →
-      G true (Some (Incoming, EAJump pc rs' mem')) (λ G', G' (AsmState (ARunning []) rs' mem' ins))
+      G true (Some (Incoming, EAJump rs' mem')) (λ G', G' (AsmState (ARunning []) rs' mem' ins))
    ).
 Proof.
   constructor => ? HG. apply steps_impl_step_end => ???.
@@ -283,7 +283,7 @@ Lemma asm_step_AWaiting_s rs mem ins:
   TStepS asm_module (AsmState AWaiting rs mem ins) (λ G,
     ∃ pc i rs' mem', rs' !!! "PC" = pc ∧
       ins !! pc = Some i ∧
-      G (Some (Incoming, EAJump pc rs' mem')) (λ G', G' (AsmState (ARunning []) rs' mem' ins))).
+      G (Some (Incoming, EAJump rs' mem')) (λ G', G' (AsmState (ARunning []) rs' mem' ins))).
 Proof.
   constructor => ??. destruct_all!. eexists _, _. split; [done|] => ? /= ?.
   apply: steps_spec_step_end. { by econs. } naive_solver.
@@ -318,7 +318,7 @@ Global Hint Resolve asm_step_AHalted_i : tstep.
 
 (** * closing *)
 Inductive asm_closed_event : Type :=
-| EACStart (pc : Z) (rs : gmap string Z) (mem : gmap Z (option Z))
+| EACStart (rs : gmap string Z) (mem : gmap Z (option Z))
 | EACSyscallCall (args : list Z)
 | EACSyscallRet (ret : Z)
 | EACPagefault (a : Z)
@@ -334,9 +334,8 @@ Definition asm_closed_pre (e : asm_closed_event) (s : bool) :
     end
   else
     match e with
-    | EACStart pc rs mem =>
-        pp_prop (rs !!! "PC" = pc) $
-        pp_end ((Incoming, EAJump pc rs mem), true)
+    | EACStart rs mem =>
+        pp_end ((Incoming, EAJump rs mem), true)
     | _ => pp_prop False (pp_quant $ λ e', pp_end e')
     end
 .
@@ -375,11 +374,10 @@ Definition asm_prod_filter (ins1 ins2 : gset Z) : seq_product_state → option s
   λ p s e p' s' e',
     e' = e ∧
     match e with
-    | EAJump pc rs mem =>
+    | EAJump rs mem =>
         s = None ∧
         s' = None ∧
-        p' = (if bool_decide (pc ∈ ins1) then SPLeft else if bool_decide (pc ∈ ins2) then SPRight else SPNone) ∧
-        rs !!! "PC" = pc ∧
+        p' = (if bool_decide (rs !!! "PC" ∈ ins1) then SPLeft else if bool_decide (rs !!! "PC" ∈ ins2) then SPRight else SPNone) ∧
         p ≠ p'
     | EASyscallCall _ =>
         s = None ∧
@@ -472,7 +470,7 @@ Proof.
       tstep_both => *. tstep_s => *. split!; [|done|]; [done|].
       tstep_s. split!. tend. apply: Hloop; [done|]. naive_solver.
   - tstep_i => pc???? Hin.
-    tstep_s. eexists (EAJump _ _ _). split!.
+    tstep_s. eexists (EAJump _ _). split!.
     { move: Hin => /lookup_union_Some_raw[?|[??]]; simplify_eq; by simpl_map_decide. }
     move: Hin => /lookup_union_Some_raw[?|[??]]; simplify_eq; simpl_map_decide.
     all: tstep_s; split!; apply: Hloop; naive_solver.
@@ -691,33 +689,31 @@ Local Ltac go_i :=
 (* TODO: Get rid of Some in recursive call (maybe by passing an itree to t instead of the +'? ) *)
 (* TODO: prove merging of two asm loops (should just be all choice between the two implementations ) *)
 Definition asm_loop (ins : list Z)
-   (t : Z → gmap string Z → gmap Z (option Z) → itree (callE
-     (option (Z * gmap string Z * gmap Z (option Z))) (Z * gmap string Z * gmap Z (option Z)) +' moduleE asm_event unit) (Z * gmap string Z * gmap Z (option Z)))
+   (t : gmap string Z → gmap Z (option Z) → itree (callE
+     (option (gmap string Z * gmap Z (option Z))) (gmap string Z * gmap Z (option Z)) +' moduleE asm_event unit) (gmap string Z * gmap Z (option Z)))
   : itree (moduleE asm_event unit) unit :=
   rec (λ a,
-    '(pc, rs, mem) ← (
-       if a is Some (npc, nrs, nmem) then
-         if bool_decide (npc ∈ ins) then
-           Ret (npc, nrs, nmem)
+    '(rs, mem) ← (
+       if a is Some (nrs, nmem) then
+         if bool_decide (nrs !!! "PC" ∈ ins) then
+           Ret (nrs, nmem)
          else
-           translate (inr_) (TVis (Outgoing, EAJump npc nrs nmem));;;;
-           pc ← translate (inr_) (TExist Z);;;
+           translate (inr_) (TVis (Outgoing, EAJump nrs nmem));;;;
            rs ← translate (inr_) (TExist _);;;
            mem ← translate (inr_) (TExist _);;;
-           translate (inr_) (TVis (Incoming, EAJump pc rs mem));;;;
-           Ret (pc, rs, mem)
+           translate (inr_) (TVis (Incoming, EAJump rs mem));;;;
+           Ret (rs, mem)
         else
-          pc ← translate (inr_) (TExist Z);;;
           rs ← translate (inr_) (TExist _);;;
           mem ← translate (inr_) (TExist _);;;
-          translate (inr_) (TVis (Incoming, EAJump pc rs mem));;;;
-          Ret (pc, rs, mem)
+          translate (inr_) (TVis (Incoming, EAJump rs mem));;;;
+          Ret (rs, mem)
      );;;
-    translate (inr_) (TAssert (pc ∈ ins));;;;
+    translate (inr_) (TAssert (rs !!! "PC" ∈ ins));;;;
     (* The env can choose if this call should be treated as a call or a return. *)
     b ← translate (inr_) (TAll bool);;;
-    if b then Ret (pc, rs, mem) else
-      r ← t pc rs mem;;;
+    if b then Ret (rs, mem) else
+      r ← t rs mem;;;
       call (Some r)
     ) None;;;; TUb.
 
@@ -731,38 +727,38 @@ Lemma tsim_asm_loop n b rs mem ins t insaddrs:
          mem1'' = mem2'' →
          rs1'' !!! "PC" = pc'' →
           (∀ pc''' rs''' mem''' i,
-              rs''' !!! "PC" = pc''' → ins !! pc''' = Some i →
-              AsmState (ARunning i) rs''' mem''' ins ⪯{asm_module, mod_itree asm_event (), n, b} (h' (pc''', rs''', mem'''), ())) →
+              rs''' !!! "PC" = pc''' →
+              ins !! pc''' = Some i →
+              AsmState (ARunning i) rs''' mem''' ins ⪯{asm_module, mod_itree asm_event (), n, b} (h' (rs''', mem'''), ())) →
           (AsmState (ARunning []) rs1'' mem1'' ins)
             ⪯{asm_module, mod_itree asm_event (), n, true}
-          (y ← rec rc (Some (pc'', rs2'', mem2''));;; h' y, ())) →
+          (y ← rec rc (Some (rs2'', mem2''));;; h' y, ())) →
       (∀ pc rs1 rs2 mem1 mem2,
           rs1 = rs2 →
           mem1 = mem2 →
           rs1 !!! "PC" = pc →
-          tsim n true asm_module (mod_itree asm_event ()) (AsmState (ARunning []) rs1 mem1 ins) tnil (k (pc, rs2, mem2), ())) →
+          tsim n true asm_module (mod_itree asm_event ()) (AsmState (ARunning []) rs1 mem1 ins) tnil (k (rs2, mem2), ())) →
     AsmState (ARunning i) rs' mem' ins ⪯{asm_module, mod_itree asm_event (), n, true}
-       (r ← interp (recursive rc) (t pc' rs' mem');;; k r, ())) →
+       (r ← interp (recursive rc) (t rs' mem');;; k r, ())) →
   (** Then we can prove an asm_loop *)
   AsmState AWaiting rs mem ins ⪯{asm_module, mod_itree asm_event (), n, b} (asm_loop insaddrs t, ()).
 Proof.
   rewrite /asm_loop => Hins Hl. set rc := (X in (rec X)).
   apply (tsim_remember_rec (mi:=asm_module)
    (λ a σi s,
-     if a is Some (pc, rs, mem) then
-       σi = AsmState (ARunning []) rs mem ins ∧ rs !!! "PC" = pc
+     if a is Some (rs, mem) then
+       σi = AsmState (ARunning []) rs mem ins
      else
        ∃ rs mem, σi = AsmState AWaiting rs mem ins
    )
-   (λ σi '(pc, rs, mem) s', ∃ i, σi = AsmState (ARunning i) rs mem ins ∧ rs !!! "PC" = pc ∧ ins !! pc = Some i)).
+   (λ σi '(rs, mem) s', ∃ i, σi = AsmState (ARunning i) rs mem ins ∧ ins !! (rs !!! "PC") = Some i)).
   { naive_solver. }
   { move => ????. go_s. done. }
   move => {}n _ Hloop σi [] CONT a Ha HCONT.
-  destruct a as [[[pc' rs'] mem']|]. 2: {
+  destruct a as [[rs' mem']|]. 2: {
     move: Ha => [{}rs [{}mem ?]]. subst.
     tstep_i => pc i {}rs {}mem HPC Hi.
     rewrite {1}rec_as_interp {2}/rc.
-    go_s. eexists _. go.
     go_s. eexists _. go.
     go_s. eexists _. go.
     go_s. split; [done|]. go.
@@ -773,12 +769,12 @@ Proof.
     revert select (eqit eq _ _ _ _) => ->. rewrite interp_bind bind_bind.
     apply: Hl; [done..| |].
     - move => ??????????. subst. apply Hloop; [done|].
-      move => ? [[rs' pc'] mem'] []. naive_solver.
+      move => ? [rs' mem'] []. naive_solver.
     - move => ????????. rewrite interp_recursive_call.
       apply Hloop. { naive_solver. }
-      move => ? [[??]?] [] [?[??]]. apply: HCONT. naive_solver.
+      move => ? [??] [] [?[??]]. apply: HCONT. naive_solver.
   }
-  destruct Ha. simplify_eq.
+  simplify_eq.
   tstep_i => pc HPC. simplify_eq.
   case_match.
   - rewrite {1}rec_as_interp {2}/rc. rewrite bool_decide_true. 2: { apply Hins. naive_solver. }
@@ -788,14 +784,13 @@ Proof.
     revert select (eqit eq _ _ _ _) => ->. rewrite interp_bind bind_bind.
     apply: Hl; [done..| |].
     + move => ??????????. subst. apply Hloop; [done|].
-      move => ? [[??] ?] []. naive_solver.
+      move => ? [? ?] []. naive_solver.
     + move => ????????. rewrite interp_recursive_call.
       apply Hloop. { naive_solver. }
-      move => ? [[??]?] [] [?[??]]. apply: HCONT. naive_solver.
+      move => ? [??] [] [?[??]]. apply: HCONT. naive_solver.
   - rewrite {1}rec_as_interp {2}/rc. rewrite bool_decide_false. 2: { move => /Hins[??]. naive_solver. }
     go_s. split; [done|]. go.
     tstep_i => pc i {}rs {}mem HPC Hi.
-    go_s. eexists _. go.
     go_s. eexists _. go.
     go_s. eexists _. go.
     go_s. split; [done|]. go.
@@ -806,10 +801,10 @@ Proof.
     revert select (eqit eq _ _ _ _) => ->. rewrite interp_bind bind_bind.
     apply: Hl; [done..| |].
     + move => ??????????. subst. apply Hloop; [done|].
-      move => ? [[??] ?] []. naive_solver.
+      move => ? [? ?] []. naive_solver.
     + move => ????????. rewrite interp_recursive_call.
       apply Hloop. { naive_solver. }
-      move => ? [[??]?] [] [?[??]]. apply: HCONT. naive_solver.
+      move => ? [??] [] [?[??]]. apply: HCONT. naive_solver.
 Qed.
 
 Module asm_examples.
@@ -826,10 +821,10 @@ Module asm_examples.
       ] ]> $ ∅.
 
   Definition itree_mul : itree (moduleE asm_event unit) unit :=
-    asm_loop [100; 101] (λ pc rs mem,
-       if bool_decide (pc = 100) then
-         Ret ((rs !!! "R30"), (<["PC":=(rs !!! "R30")]> $ <["R1":=(rs !!! "R1") * (rs !!! "R2")]> $ rs), mem)
-       else if bool_decide (pc = 101) then
+    asm_loop [100; 101] (λ rs mem,
+       if bool_decide (rs !!! "PC" = 100) then
+         Ret ((<["PC":=(rs !!! "R30")]> $ <["R1":=(rs !!! "R1") * (rs !!! "R2")]> $ rs), mem)
+       else if bool_decide (rs !!! "PC" = 101) then
          translate (inr_) TUb
        else
          translate (inr_) TNb
@@ -857,7 +852,7 @@ Module asm_examples.
     tstep_i => ??; simplify_map_eq'.
     tstep_i; simplify_map_eq'. split!.
     revert select (eqit eq _ _ _ _) => ->.
-    apply HCONT; simplify_map_eq' => //.
+    apply: HCONT; simplify_map_eq' => //.
   Qed.
 
   Definition asm_mul_client : gmap Z asm_instr :=
@@ -888,21 +883,21 @@ Module asm_examples.
       ] ]> $ ∅.
 
   Definition itree_mul_client : itree (moduleE asm_event unit) unit :=
-    asm_loop [200; 201; 202; 203; 204] (λ pc rs mem,
-       if bool_decide (pc = 200) then
+    asm_loop [200; 201; 202; 203; 204] (λ rs mem,
+       if bool_decide (rs !!! "PC" = 200) then
          r29' ← translate (inr_) (TExist Z);;;
          (* translate (inr_) (TVis (EAJump 100 (<["PC":=100]> $ <["R30":= 212]> $ <["R29":= r29']> $ <["R2":= 2]> $ <["R1":= 2]> $ rs)));;;; *)
-         '(pc', rs', mem') ← call (Some (100, (<["PC":=100]> $ <["R30":= 203]> $ <["R29":= r29']> $ <["R2":= 2]> $ <["R1":= 2]> $ rs), mem));;;
-         translate (inr_) (TAssume (pc' = 203));;;;
+         '(rs', mem') ← call (Some ((<["PC":=100]> $ <["R30":= 203]> $ <["R29":= r29']> $ <["R2":= 2]> $ <["R1":= 2]> $ rs), mem));;;
+         translate (inr_) (TAssume (rs' !!! "PC" = 203));;;;
          translate (inr_) (TAssume (rs' !!! "R29" = r29'));;;;
          translate (inr_) (TAssume ((rs !!! "R30") ≠ 200 ∧ (rs !!! "R30") ≠ 201 ∧ (rs !!! "R30") ≠ 202 ∧ (rs !!! "R30") ≠ 203 ∧ (rs !!! "R30") ≠ 204));;;;
          r30' ← translate (inr_) (TExist Z);;;
          (* translate (inr_) (TVis (EAJump r30 (<["PC":= r30]> $ <["R30":= r30']> rs')));;;; *)
-         Ret ((rs !!! "R30"), (<["PC":= (rs !!! "R30")]> $ <["R30":= r30']> rs'), mem')
-       else if bool_decide (pc = 201) then translate (inr_) TUb
-       else if bool_decide (pc = 202) then translate (inr_) TUb
-       else if bool_decide (pc = 203) then translate (inr_) TUb
-       else if bool_decide (pc = 204) then translate (inr_) TUb
+         Ret ((<["PC":= (rs !!! "R30")]> $ <["R30":= r30']> rs'), mem')
+       else if bool_decide (rs !!! "PC" = 201) then translate (inr_) TUb
+       else if bool_decide (rs !!! "PC" = 202) then translate (inr_) TUb
+       else if bool_decide (rs !!! "PC" = 203) then translate (inr_) TUb
+       else if bool_decide (rs !!! "PC" = 204) then translate (inr_) TUb
        else translate (inr_) TNb
     ).
 
@@ -921,20 +916,20 @@ Module asm_examples.
     move: Hi. rewrite !lookup_insert_Some !lookup_empty => Hi. destruct_all!; simplify_eq.
     all: repeat (rewrite bool_decide_false; [|done]); rewrite bool_decide_true //.
     all: try by go_s.
-    tstep_i; simplify_map_eq'. split!.
-    tstep_i; simplify_map_eq'. split!.
-    tstep_i; simplify_map_eq'. split!.
+    tstep_i; simplify_map_eq'.
+    tstep_i; simplify_map_eq'.
+    tstep_i; simplify_map_eq'.
     tstep_i => ??; simplify_map_eq'.
-    tstep_i; simplify_map_eq'. split!.
-    tstep_i; simplify_map_eq'. split!.
+    tstep_i; simplify_map_eq'.
+    tstep_i; simplify_map_eq'.
     tstep_i => ??; simplify_map_eq'.
-    tstep_i; simplify_map_eq'. split!.
-    tstep_i; simplify_map_eq'. split!.
+    tstep_i; simplify_map_eq'. 
+    tstep_i; simplify_map_eq'.
     sort_map_insert; simplify_map_eq'.
     go_s. eexists (rs !!! "R30"); go.
     go_s.
     revert select (eqit eq _ _ _ _) => ->.
-    apply Hloop. { by sort_map_insert. } { done. } { by simplify_map_eq'. }
+    apply: Hloop. { by sort_map_insert. } { done. } { by simplify_map_eq'. }
     move => pc' rs'' mem'' i HPC' Hi'.
     go_s => ?; go; subst. unfold asm_mul_client in Hi'. simplify_map_eq.
     go_s => ?; go.
@@ -946,6 +941,6 @@ Module asm_examples.
     tstep_i; simplify_map_eq'. split!.
     go_s. eexists _; go.
     go_s. revert select (eqit eq _ _ _ _) => ->.
-    apply HCONT; by simplify_map_eq'.
+    apply: HCONT; by simplify_map_eq'.
   Qed.
 End asm_examples.
